Core/Typing.v
@@ -1,4 +1,5 @@
 From Stdlib Require Import Arith.PeanoNat.
+From Stdlib Require Import Strings.String.
 From DOMLCore Require Import Syntax Context Substitution.
 
 Inductive value : tm -> Prop :=
@@ -19,104 +20,122 @@ Inductive value : tm -> Prop :=
 | V_Inl : forall U v, value v -> value (tInl U v)
 | V_Inr : forall T v, value v -> value (tInr T v)
 | V_Eq : forall T e1 e2, value (tEq T e1 e2)
-| V_Refl : forall v, value v -> value (tRefl v)
-| V_Dom : forall d, value (tDom d)
-| V_IntroDom : forall d args proof,
-    value args -> value proof -> value (tIntroDom d args proof).
+| V_Refl : forall v, value v -> value (tRefl v).
 
-Inductive has_type : dom_context -> context -> tm -> tm -> Prop :=
-| T_Sort : forall Delta Gamma s,
-    has_type Delta Gamma (tSort s) (tSort (S s))
-| T_Bool : forall Delta Gamma,
-    has_type Delta Gamma tBool (tSort 0)
-| T_Int : forall Delta Gamma,
-    has_type Delta Gamma tInt (tSort 0)
-| T_Unit : forall Delta Gamma,
-    has_type Delta Gamma tUnit (tSort 0)
-| T_Empty : forall Delta Gamma,
-    has_type Delta Gamma tEmpty (tSort 0)
-| T_True : forall Delta Gamma,
-    has_type Delta Gamma tTrue tBool
-| T_False : forall Delta Gamma,
-    has_type Delta Gamma tFalse tBool
-| T_IntLit : forall Delta Gamma z,
-    has_type Delta Gamma (tIntLit z) tInt
-| T_UnitLit : forall Delta Gamma,
-    has_type Delta Gamma tUnitLit tUnit
-| T_Var : forall Delta Gamma x T,
+Inductive defeq : tm -> tm -> Prop :=
+| DE_Refl : forall T, defeq T T.
+
+Inductive has_type : dom_context -> const_context -> context -> tm -> tm -> Prop :=
+| T_Sort : forall Delta Omega Gamma s,
+    has_type Delta Omega Gamma (tSort s) (tSort (S s))
+| T_Bool : forall Delta Omega Gamma,
+    has_type Delta Omega Gamma tBool (tSort 0)
+| T_Int : forall Delta Omega Gamma,
+    has_type Delta Omega Gamma tInt (tSort 0)
+| T_Unit : forall Delta Omega Gamma,
+    has_type Delta Omega Gamma tUnit (tSort 0)
+| T_Empty : forall Delta Omega Gamma,
+    has_type Delta Omega Gamma tEmpty (tSort 0)
+| T_True : forall Delta Omega Gamma,
+    has_type Delta Omega Gamma tTrue tBool
+| T_False : forall Delta Omega Gamma,
+    has_type Delta Omega Gamma tFalse tBool
+| T_IntLit : forall Delta Omega Gamma z,
+    has_type Delta Omega Gamma (tIntLit z) tInt
+| T_UnitLit : forall Delta Omega Gamma,
+    has_type Delta Omega Gamma tUnitLit tUnit
+| T_Var : forall Delta Omega Gamma x T,
     lookup x Gamma = Some T ->
-    has_type Delta Gamma (tVar x) T
-| T_Let : forall Delta Gamma x e1 e2 T U,
-    has_type Delta Gamma e1 T ->
-    has_type Delta (extend Gamma x T) e2 U ->
-    has_type Delta Gamma (tLet x e1 e2) U
-| T_Pi : forall Delta Gamma x T U s1 s2,
-    has_type Delta Gamma T (tSort s1) ->
-    has_type Delta (extend Gamma x T) U (tSort s2) ->
-    has_type Delta Gamma (tPi x T U) (tSort (Nat.max s1 s2))
-| T_Lam : forall Delta Gamma x T e U,
-    has_type Delta (extend Gamma x T) e U ->
-    has_type Delta Gamma (tLam x T e) (tPi x T U)
-| T_App : forall Delta Gamma e1 e2 x T U,
-    has_type Delta Gamma e1 (tPi x T U) ->
-    has_type Delta Gamma e2 T ->
-    has_type Delta Gamma (tApp e1 e2) (subst x e2 U)
-| T_Sigma : forall Delta Gamma x T U s1 s2,
-    has_type Delta Gamma T (tSort s1) ->
-    has_type Delta (extend Gamma x T) U (tSort s2) ->
-    has_type Delta Gamma (tSigma x T U) (tSort (Nat.max s1 s2))
-| T_Pair : forall Delta Gamma x e1 e2 T U,
-    has_type Delta Gamma e1 T ->
-    has_type Delta Gamma e2 (subst x e1 U) ->
-    has_type Delta Gamma (tPair e1 e2) (tSigma x T U)
-| T_Fst : forall Delta Gamma e x T U,
-    has_type Delta Gamma e (tSigma x T U) ->
-    has_type Delta Gamma (tFst e) T
-| T_Snd : forall Delta Gamma e x T U,
-    has_type Delta Gamma e (tSigma x T U) ->
-    has_type Delta Gamma (tSnd e) (subst x (tFst e) U)
-| T_Sum : forall Delta Gamma T U s1 s2,
-    has_type Delta Gamma T (tSort s1) ->
-    has_type Delta Gamma U (tSort s2) ->
-    has_type Delta Gamma (tSum T U) (tSort (Nat.max s1 s2))
-| T_Inl : forall Delta Gamma U e T s,
-    has_type Delta Gamma e T ->
-    has_type Delta Gamma U (tSort s) ->
-    has_type Delta Gamma (tInl U e) (tSum T U)
-| T_Inr : forall Delta Gamma T e U s,
-    has_type Delta Gamma e U ->
-    has_type Delta Gamma T (tSort s) ->
-    has_type Delta Gamma (tInr T e) (tSum T U)
-| T_Case : forall Delta Gamma e x el y er T U R,
-    has_type Delta Gamma e (tSum T U) ->
-    has_type Delta (extend Gamma x T) el R ->
-    has_type Delta (extend Gamma y U) er R ->
-    has_type Delta Gamma (tCase e x el y er) R
-| T_Eq : forall Delta Gamma T e1 e2 s,
-    has_type Delta Gamma T (tSort s) ->
-    has_type Delta Gamma e1 T ->
-    has_type Delta Gamma e2 T ->
-    has_type Delta Gamma (tEq T e1 e2) (tSort 0)
-| T_Refl : forall Delta Gamma e T,
-    has_type Delta Gamma e T ->
-    has_type Delta Gamma (tRefl e) (tEq T e e)
-| T_Dom : forall Delta Gamma d ent,
+    has_type Delta Omega Gamma (tVar x) T
+| T_Const : forall Delta Omega Gamma c T,
+    lookup c Omega = Some T ->
+    has_type Delta Omega Gamma (tConst c) T
+| T_Let : forall Delta Omega Gamma x e1 e2 T U s,
+    has_type Delta Omega Gamma T (tSort s) ->
+    has_type Delta Omega Gamma e1 T ->
+    has_type Delta Omega (extend Gamma x T) e2 U ->
+    has_type Delta Omega Gamma (tLet x e1 e2) (subst x e1 U)
+| T_Pi : forall Delta Omega Gamma x T U s1 s2,
+    has_type Delta Omega Gamma T (tSort s1) ->
+    has_type Delta Omega (extend Gamma x T) U (tSort s2) ->
+    has_type Delta Omega Gamma (tPi x T U) (tSort (Nat.max s1 s2))
+| T_Lam : forall Delta Omega Gamma x T e U s,
+    has_type Delta Omega Gamma T (tSort s) ->
+    has_type Delta Omega (extend Gamma x T) e U ->
+    has_type Delta Omega Gamma (tLam x T e) (tPi x T U)
+| T_App : forall Delta Omega Gamma e1 e2 x T U,
+    has_type Delta Omega Gamma e1 (tPi x T U) ->
+    has_type Delta Omega Gamma e2 T ->
+    has_type Delta Omega Gamma (tApp e1 e2) (subst x e2 U)
+| T_Sigma : forall Delta Omega Gamma x T U s1 s2,
+    has_type Delta Omega Gamma T (tSort s1) ->
+    has_type Delta Omega (extend Gamma x T) U (tSort s2) ->
+    has_type Delta Omega Gamma (tSigma x T U) (tSort (Nat.max s1 s2))
+| T_Pair : forall Delta Omega Gamma x e1 e2 T U s,
+    has_type Delta Omega Gamma (tSigma x T U) (tSort s) ->
+    has_type Delta Omega Gamma e1 T ->
+    has_type Delta Omega Gamma e2 (subst x e1 U) ->
+    has_type Delta Omega Gamma (tPair e1 e2) (tSigma x T U)
+| T_Fst : forall Delta Omega Gamma e x T U,
+    has_type Delta Omega Gamma e (tSigma x T U) ->
+    has_type Delta Omega Gamma (tFst e) T
+| T_Snd : forall Delta Omega Gamma e x T U,
+    has_type Delta Omega Gamma e (tSigma x T U) ->
+    has_type Delta Omega Gamma (tSnd e) (subst x (tFst e) U)
+| T_Sum : forall Delta Omega Gamma T U s1 s2,
+    has_type Delta Omega Gamma T (tSort s1) ->
+    has_type Delta Omega Gamma U (tSort s2) ->
+    has_type Delta Omega Gamma (tSum T U) (tSort (Nat.max s1 s2))
+| T_Inl : forall Delta Omega Gamma U e T s1 s2,
+    has_type Delta Omega Gamma T (tSort s1) ->
+    has_type Delta Omega Gamma e T ->
+    has_type Delta Omega Gamma U (tSort s2) ->
+    has_type Delta Omega Gamma (tInl U e) (tSum T U)
+| T_Inr : forall Delta Omega Gamma T e U s1 s2,
+    has_type Delta Omega Gamma e U ->
+    has_type Delta Omega Gamma T (tSort s1) ->
+    has_type Delta Omega Gamma U (tSort s2) ->
+    has_type Delta Omega Gamma (tInr T e) (tSum T U)
+| T_Case : forall Delta Omega Gamma e x el y er T U R,
+    has_type Delta Omega Gamma e (tSum T U) ->
+    has_type Delta Omega (extend Gamma x T) el R ->
+    has_type Delta Omega (extend Gamma y U) er R ->
+    has_type Delta Omega Gamma (tCase e x el y er) R
+| T_Eq : forall Delta Omega Gamma T e1 e2 s,
+    has_type Delta Omega Gamma T (tSort s) ->
+    has_type Delta Omega Gamma e1 T ->
+    has_type Delta Omega Gamma e2 T ->
+    has_type Delta Omega Gamma (tEq T e1 e2) (tSort 0)
+| T_Refl : forall Delta Omega Gamma e T s,
+    has_type Delta Omega Gamma T (tSort s) ->
+    has_type Delta Omega Gamma e T ->
+    has_type Delta Omega Gamma (tRefl e) (tEq T e e)
+| T_EqElim : forall Delta Omega Gamma P e e' p q x T s,
+    has_type Delta Omega Gamma P (tPi x T (tSort s)) ->
+    has_type Delta Omega Gamma p (tEq T e e') ->
+    has_type Delta Omega Gamma q (tApp P e) ->
+    has_type Delta Omega Gamma (tEqElim P e e' p q) (tApp P e')
+| T_DomainType : forall Delta Omega Gamma d ent s,
     lookup d Delta = Some ent ->
-    has_type Delta Gamma (tDom d) (tSort 0)
-| T_IntroDom : forall Delta Gamma d ent args proof,
+    has_type Delta Omega Gamma (elab_tree (de_tree ent)) (tSort s) ->
+    has_type Delta Omega Gamma (de_constraint ent)
+      (tPi "_args"%string (elab_tree (de_tree ent)) tBool) ->
+    has_type Delta Omega Gamma (domain_type ent) (tSort 0)
+| T_IntroDom : forall Delta Omega Gamma d ent args proof s,
     lookup d Delta = Some ent ->
-    has_type Delta Gamma args (elab_tree (de_tree ent)) ->
-    has_type Delta Gamma proof
+    has_type Delta Omega Gamma (domain_type ent) (tSort s) ->
+    has_type Delta Omega Gamma args (elab_tree (de_tree ent)) ->
+    has_type Delta Omega Gamma proof
       (tEq tBool (tApp (de_constraint ent) args) tTrue) ->
-    has_type Delta Gamma (tIntroDom d args proof) (tDom d)
-| T_Plus : forall Delta Gamma e1 e2,
-    has_type Delta Gamma e1 tInt ->
-    has_type Delta Gamma e2 tInt ->
-    has_type Delta Gamma (tPlus e1 e2) tInt
-| T_Minus : forall Delta Gamma e1 e2,
-    has_type Delta Gamma e1 tInt ->
-    has_type Delta Gamma e2 tInt ->
-    has_type Delta Gamma (tMinus e1 e2) tInt.
+    has_type Delta Omega Gamma (intro_dom args proof) (domain_type ent)
+| T_Plus : forall Delta Omega Gamma e1 e2,
+    has_type Delta Omega Gamma e1 tInt ->
+    has_type Delta Omega Gamma e2 tInt ->
+    has_type Delta Omega Gamma (tPlus e1 e2) tInt
+| T_Minus : forall Delta Omega Gamma e1 e2,
+    has_type Delta Omega Gamma e1 tInt ->
+    has_type Delta Omega Gamma e2 tInt ->
+    has_type Delta Omega Gamma (tMinus e1 e2) tInt.
 
-Hint Constructors value has_type : core.
+Hint Constructors value defeq has_type : core.
 
