Core/Automation.v
@@ -6,7 +6,7 @@ Ltac inv H := inversion H; subst; clear H.
 Ltac crush_core :=
   repeat match goal with
   | H : value (tLam _ _ _) |- _ => inv H
-  | H : has_type _ _ _ _ |- _ => progress (inversion H; subst; clear H)
+  | H : has_type _ _ _ _ _ |- _ => progress (inversion H; subst; clear H)
   | H : lookup _ (extend _ _ _) = Some _ |- _ =>
       unfold extend in H; simpl in H
   | |- context [String.eqb ?x ?x] => rewrite String.eqb_refl
