Core/Lemmas.v
@@ -4,60 +4,59 @@ From DOMLCore Require Import Syntax Context Substitution Typing Operational Auto
 Import ListNotations.
 
 Lemma canonical_bool :
-  forall Delta v,
-    has_type Delta [] v tBool ->
+  forall Delta Omega v,
+    has_type Delta Omega [] v tBool ->
     value v ->
     v = tTrue \/ v = tFalse.
 Proof.
-  intros Delta v HT HV.
+  intros Delta Omega v HT HV.
   inv HV; try solve [inv HT].
   - left; reflexivity.
   - right; reflexivity.
 Qed.
 
 Lemma canonical_int :
-  forall Delta v,
-    has_type Delta [] v tInt ->
+  forall Delta Omega v,
+    has_type Delta Omega [] v tInt ->
     value v ->
     exists z, v = tIntLit z.
 Proof.
-  intros Delta v HT HV.
+  intros Delta Omega v HT HV.
   inv HV; try solve [inv HT].
   exists z. reflexivity.
 Qed.
 
 Lemma canonical_pi :
-  forall Delta v x T U,
-    has_type Delta [] v (tPi x T U) ->
+  forall Delta Omega v x T U,
+    has_type Delta Omega [] v (tPi x T U) ->
     value v ->
     exists e, v = tLam x T e.
 Proof.
-  intros Delta v x T U HT HV.
+  intros Delta Omega v x T U HT HV.
   inv HV; try solve [inv HT].
   inv HT.
   exists e. reflexivity.
 Qed.
 
 Lemma canonical_sigma :
-  forall Delta v x T U,
-    has_type Delta [] v (tSigma x T U) ->
+  forall Delta Omega v x T U,
+    has_type Delta Omega [] v (tSigma x T U) ->
     value v ->
     exists v1 v2, v = tPair v1 v2 /\ value v1 /\ value v2.
 Proof.
-  intros Delta v x T U HT HV.
+  intros Delta Omega v x T U HT HV.
   inv HV; try solve [inv HT].
-  inv HT.
-  exists v1, v2. repeat split; eauto.
+  inv HT; exists v1, v2; repeat split; eauto.
 Qed.
 
 Lemma canonical_sum :
-  forall Delta v T U,
-    has_type Delta [] v (tSum T U) ->
+  forall Delta Omega v T U,
+    has_type Delta Omega [] v (tSum T U) ->
     value v ->
     (exists v1, v = tInl U v1 /\ value v1) \/
     (exists v2, v = tInr T v2 /\ value v2).
 Proof.
-  intros Delta v T U HT HV.
+  intros Delta Omega v T U HT HV.
   inversion HV; subst; try solve [inversion HT].
   - inversion HT; subst.
     left. eexists. split; [reflexivity | eauto].
@@ -65,11 +64,22 @@ Proof.
     right. eexists. split; [reflexivity | eauto].
 Qed.
 
+Lemma canonical_eq_proof :
+  forall Delta Omega v T e e',
+    has_type Delta Omega [] v (tEq T e e') ->
+    value v ->
+    exists w, v = tRefl w /\ e = w /\ e' = w /\ value w.
+Proof.
+  intros Delta Omega v T e e' HT HV.
+  inversion HV; subst; try solve [inversion HT].
+  inversion HT; subst. eexists. repeat split; eauto.
+Qed.
+
 Lemma substitution_preserves_typing :
-  forall Delta Gamma x U e v T,
-    has_type Delta (extend Gamma x U) e T ->
-    has_type Delta Gamma v U ->
-    has_type Delta Gamma (subst x v e) T.
+  forall Delta Omega Gamma x U e v T,
+    has_type Delta Omega (extend Gamma x U) e T ->
+    has_type Delta Omega Gamma v U ->
+    has_type Delta Omega Gamma (subst x v e) T.
 Proof.
   (**
     The actual proof is by induction on the first typing derivation.  The
