Core/Metatheory.v
@@ -5,9 +5,11 @@ Import ListNotations.
 
 Theorem preservation :
   forall Delta e e' T,
-    has_type Delta [] e T ->
+    has_type Delta [] [] e T ->
     step e e' ->
-    has_type Delta [] e' T.
+    exists T',
+      has_type Delta [] [] e' T' /\
+      defeq T T'.
 Proof.
   (**
     Standard induction on the reduction derivation.  The beta and let cases
@@ -19,13 +21,83 @@ Admitted.
 
 Theorem progress :
   forall Delta e T,
-    has_type Delta [] e T ->
+    has_type Delta [] [] e T ->
     value e \/ exists e', step e e'.
 Proof.
-  (**
-    Standard induction on typing.  Canonical-form lemmas handle elimination
-    forms over values; congruence rules handle reducible subterms.  Domain
-    introductions are values once their argument and proof fields are values.
-   *)
-Admitted.
+  intros Delta e T HT.
+  remember (@nil (const_name * tm)) as Omega eqn:HOmega.
+  remember (@nil (var * tm)) as Gamma eqn:HGamma.
+  induction HT; subst; eauto with core; try discriminate.
+  - right. destruct IHHT2; auto.
+    + eauto with core.
+    + destruct H as [e1' Hstep]. eauto with core.
+  - right. destruct IHHT1; auto.
+    + destruct IHHT2; auto.
+      * destruct (canonical_pi Delta [] e1 x T U HT1 H) as [body Heq].
+        subst. eauto with core.
+      * destruct H0 as [e2' Hstep]. eauto with core.
+    + destruct H as [e1' Hstep]. eauto with core.
+  - destruct (IHHT2 eq_refl eq_refl) as [Hv1 | [e1' Hstep1]].
+    + destruct (IHHT3 eq_refl eq_refl) as [Hv2 | [e2' Hstep2]].
+      * left. constructor; assumption.
+      * right. exists (tPair e1 e2'). constructor; assumption.
+    + right. exists (tPair e1' e2). constructor; assumption.
+  - right. destruct IHHT; auto.
+    + destruct (canonical_sigma Delta [] e x T U HT H)
+        as [v1 [v2 [Heq [Hv1 Hv2]]]].
+      subst. eauto with core.
+    + destruct H as [e' Hstep]. eauto with core.
+  - right. destruct IHHT; auto.
+    + destruct (canonical_sigma Delta [] e x T U HT H)
+        as [v1 [v2 [Heq [Hv1 Hv2]]]].
+      subst. eauto with core.
+    + destruct H as [e' Hstep]. eauto with core.
+  - destruct (IHHT2 eq_refl eq_refl) as [Hv | [e' Hstep]].
+    + left. constructor. assumption.
+    + right. exists (tInl U e'). constructor. assumption.
+  - destruct (IHHT1 eq_refl eq_refl) as [Hv | [e' Hstep]].
+    + left. constructor. assumption.
+    + right. exists (tInr T e'). constructor. assumption.
+  - right. destruct IHHT1; auto.
+    + destruct (canonical_sum Delta [] e T U HT1 H) as
+        [[v1 [Heq Hv1]] | [v2 [Heq Hv2]]].
+      * subst. eauto with core.
+      * subst. eauto with core.
+    + destruct H as [e' Hstep]. eauto with core.
+  - destruct (IHHT2 eq_refl eq_refl) as [Hv | [e0' Hstep]].
+    + left. constructor. assumption.
+    + right. exists (tRefl e0'). constructor. assumption.
+  - right.
+    destruct (IHHT2 eq_refl eq_refl) as [Hvp | [p' Hstepp]].
+    + destruct (IHHT3 eq_refl eq_refl) as [Hvq | [q' Hstepq]].
+      * destruct (canonical_eq_proof Delta [] p T e e' HT2 Hvp)
+          as [w [Hp [He [He' Hvw]]]].
+        subst. exists q. constructor. assumption.
+      * exists (tEqElim P e e' p q'). constructor; assumption.
+    + exists (tEqElim P e e' p' q). constructor. assumption.
+  - left. unfold domain_type. constructor.
+  - destruct (IHHT2 eq_refl eq_refl) as [HvArgs | [args' HstepArgs]].
+    + destruct (IHHT3 eq_refl eq_refl) as [HvProof | [proof' HstepProof]].
+      * left. unfold intro_dom. constructor; assumption.
+      * right. exists (intro_dom args proof').
+        unfold intro_dom. constructor; assumption.
+    + right. exists (intro_dom args' proof).
+      unfold intro_dom. constructor; assumption.
+  - right.
+    destruct (IHHT1 eq_refl eq_refl) as [Hv1 | [e1' Hstep1]].
+    + destruct (IHHT2 eq_refl eq_refl) as [Hv2 | [e2' Hstep2]].
+      * destruct (canonical_int Delta [] _ HT1 Hv1) as [z1 Heq1].
+        destruct (canonical_int Delta [] _ HT2 Hv2) as [z2 Heq2].
+        subst. eauto with core.
+      * eexists. eapply ST_Plus2; eauto.
+    + eexists. eapply ST_Plus1; eauto.
+  - right.
+    destruct (IHHT1 eq_refl eq_refl) as [Hv1 | [e1' Hstep1]].
+    + destruct (IHHT2 eq_refl eq_refl) as [Hv2 | [e2' Hstep2]].
+      * destruct (canonical_int Delta [] _ HT1 Hv1) as [z1 Heq1].
+        destruct (canonical_int Delta [] _ HT2 Hv2) as [z2 Heq2].
+        subst. eauto with core.
+      * eexists. eapply ST_Minus2; eauto.
+    + eexists. eapply ST_Minus1; eauto.
+Qed.
 
