README.md
@@ -2,6 +2,10 @@
 
 注意，`coqc`编译器已经升级命名为`rocq`
 
+## Structure
+
+
+
 ## Setup
 
 To use this project, you will need to install some specific dependencies.
